---
title: "DATA605 Homework 14"
author: "Henry Otuadinma"
date: "01/12/2019"
output: html_document
---

```{r setup, include=FALSE}
knitr::opts_chunk$set(echo = TRUE)
```

#### This week, we'll work out some Taylor Series expansions of popular functions.
1. $f(x) = \frac{1}{(1-x)}$
2. $f(x) = e^x$
3. $f(x) = ln(1 + x)$

#### For each function, only consider its valid ranges as indicated in the notes when you are computing the Taylor Series expansion.

Solutions:

From Taylor's series:

$P(x)=f(0)+f′(0)(x)+f′′(0)\frac{x^2}{2!} + f(3)(0)\frac{x^3}{3!}+....+f(n)(0)\frac{x^n}{n!}$

1. $f(x) = \frac{1}{(1-x)}, f(0) = 1$
  
  $f^1(x) = \frac{1}{(1-x)^2}, f^1(0) = 1$
  
  $f^2(x) = \frac{2}{(1-x)^3}, f^2(0) = 2$
  
  $f^3(x) = \frac{6}{(1-x)^4}, f3(0) = 6$
  
  $f^4(x) = \frac{24}{(1-x)^5}, f^4(0) = 24$
  
  $f^5(x) = \frac{120}{(1-x)^6}, f^5(0) = 120$
  
  => $\frac{1}{(1 - x)} = 1 + x + \frac{2x^2}{2!} + \frac{6x^3}{3!} + \frac{24x^4}{4!} + \frac{120x^5}{5!} + ...$
  $= 1 + x + x^2 + x^3 + x^4 + x^5 + ...$


2. $f(x) = e^x$
  
   $f(x)=e^x, f(0)=e^0 = 1$

  $f'(x)=ex, f'(0)=e0 = 1$

  $f''(x)=e^x , f''(0)=e^0 = 1$

  $f^{(3)}(x)=e^x , f^{(3)}(0)=e^0 = 1$

  $f^{(4)}(x)=e^x , f(4)(0)=e^0 = 1$

  $f^{(5)}(x)=e^x , f^{(5)}(0)=e^0 = 1$

  $f^{(n)}(x)=e^x , f^{(n)}(0)=e^0 = 1$

  $.$
  $.$
  $.$

  $f^{(n)}(x)=e^x , f^{(n)}(0)=e^0 = 1$
  
  => $e^x = 1 + x + \frac{x^2}{2!} + \frac{x^3}{3!} + \frac{x^4}{4!} + \frac{x^5}{5!} ...  + \frac{x^n}{n!}$




3. $f(x) = ln(1 + x)$

setting $u=1+x$ => $\frac{du}{dx}=1 => dx=\frac{1}{u}du$

$f′(x)=\frac{1}{u} *1$

=> $f′(x)=\frac{1}{1+x}$

$f'0(x)=ln(1+x)=0$

$f′0(x)=ln(1+x)=1$

$f′′0(x)=ln(1+x)=−1$

$f^{(3)}0(x)=ln(1+x)=2$

$f^{(4)}0(x)=ln(1+x)=−6$

$f^{(5)}0(x)=ln(1+x)=24$

From Taylor’s Series, this can be represented as: 

$x−\frac{x^2}{2}+\frac{x^3}{3}−\frac{x^4}{4} + \frac{x^5}{5} +...+$











































































